examples/hoare_logic/blocking_semantics3/blocking_semantics3_WP_progress_1.v
@@ -678,5 +678,3 @@ do 3 eexists.
 econstructor.
 eauto.
 Qed.
-
-
