examples/hoare_logic/blocking_semantics5/blocking_semantics5_WP_wp_reduction_3.v
@@ -527,35 +527,46 @@ Axiom abstract_effects_writes : forall (sigma:(map mident value)) (pi:(list
   (abstract_effects s q)) -> (eval_fmla sigma pi (wp s (abstract_effects s
   q))).
 
-Require Import Why3.
-Ltac ae := why3 "alt-ergo" timelimit 3.
+Axiom monotonicity : forall (s:stmt) (p:fmla) (q:fmla),
+  (valid_fmla (Fimplies p q)) -> (valid_fmla (Fimplies (wp s p) (wp s q))).
+
+Axiom distrib_conj : forall (s:stmt) (sigma:(map mident value)) (pi:(list
+  (ident* value)%type)) (p:fmla) (q:fmla), ((eval_fmla sigma pi (wp s p)) /\
+  (eval_fmla sigma pi (wp s q))) -> (eval_fmla sigma pi (wp s (Fand p q))).
 
 (* Why3 goal *)
-Theorem monotonicity : forall (s:stmt),
+Theorem wp_reduction : forall (sigma:(map mident value)) (sigma':(map mident
+  value)) (pi:(list (ident* value)%type)) (pi':(list (ident* value)%type))
+  (s:stmt),
   match s with
   | Sskip => True
-  | (Sassign m t) => forall (p:fmla) (q:fmla), (valid_fmla (Fimplies p q)) ->
-      (valid_fmla (Fimplies (wp s p) (wp s q)))
+  | (Sassign m t) => True
   | (Sseq s1 s2) => True
   | (Sif t s1 s2) => True
   | (Sassert f) => True
-  | (Swhile t f s1) => True
+  | (Swhile t f s1) => (forall (s':stmt), (one_step sigma pi s1 sigma' pi'
+      s') -> forall (q:fmla), (eval_fmla sigma pi (wp s1 q)) ->
+      (eval_fmla sigma' pi' (wp s' q))) -> forall (s':stmt), (one_step sigma
+      pi s sigma' pi' s') -> forall (q:fmla), (eval_fmla sigma pi (wp s
+      q)) -> (eval_fmla sigma' pi' (wp s' q))
   end.
 destruct s; auto.
-unfold valid_fmla.
 simpl.
-intros.
-apply eval_msubst.
-apply fresh_from_fmla.
-rewrite eval_msubst in H0.
-rewrite get_stack_eq; auto.
-rewrite get_stack_eq in H0; auto.
-apply eval_change_free.
-apply fresh_from_fmla.
-rewrite eval_change_free in H0.
-apply H; auto.
-apply fresh_from_fmla.
-apply fresh_from_fmla.
+intros H s' H1 q (_ & H3).
+apply abstract_effects_generalize in H3; simpl in H3.
+inversion H1; subst; auto.
+simpl.
+apply distrib_conj.
+split.
+apply H3; auto.
+apply abstract_effects_writes.
+apply abstract_effects_monotonic with (sigma := sigma') (pi := pi').
+simpl; auto.
+(* false *)
+apply H3.
+split; auto.
+rewrite H11; auto.
+easy.
 Qed.
 
 
